examples/rel/Benton2004.Aux.fst
@@ -1,0 +1,11 @@
+module Benton2004.Aux
+
+type rel (t: Type0) = t -> t -> GTot Type0
+
+(* NOTE: I define this `holds` abstract here to prevent Z3 from looping. *)
+
+abstract let holds (#t: Type0) (p: rel t) (s s' : t) : GTot Type0 =
+  p s s'
+abstract let holds_equiv (#t: Type0) (p: rel t) (s s' : t) : Lemma
+  (holds p s s' <==> p s s')
+= ()
